Weidenbach_Book/CDCL_W_Implementation.thy
@@ -1,5 +1,5 @@
-theory CDCL_CW_Implementation
-imports DPLL_CDCL_Implementation CDCL_CW_Termination
+theory CDCL_W_Implementation
+imports DPLL_CDCL_W_Implementation CDCL_W_Termination
 begin
 
 notation image_mset (infixr "`#" 90)
@@ -1623,7 +1623,7 @@ fun max A_ (Set.Set (x :: xs)) =
 
 end; (*struct Lattices_Big*)
 
-structure CDCL_CW : sig
+structure CDCL_W : sig
   datatype 'a conflicting_clause = C_True | C_Clause of 'a
   val equal_conflicting_clause : 'a HOL.equal -> 'a conflicting_clause HOL.equal
   val get_rev_level :
@@ -1666,7 +1666,7 @@ fun get_maximum_level A_ d m =
         (Multiset.image_mset
           (fn l => get_rev_level A_ l Arith.zero_nat (List.rev m)) d)));
 
-end; (*struct CDCL_CW*)
+end; (*struct CDCL_W*)
 
 structure Product_Type : sig
   val equal_proda : 'a HOL.equal -> 'b HOL.equal -> 'a * 'b -> 'a * 'b -> bool
@@ -1680,7 +1680,7 @@ fun equal_prod A_ B_ = {equal = equal_proda A_ B_} : ('a * 'b) HOL.equal;
 
 end; (*struct Product_Type*)
 
-structure CDCL_CW_Implementation : sig
+structure CDCL_W_Implementation : sig
   datatype cdcl_state_inv_I =
   ConI of
     ((Arith.nat, Arith.nat, (Arith.nat Clausal_Logic.literal list))
@@ -1689,7 +1689,7 @@ structure CDCL_CW_Implementation : sig
         ((Arith.nat Clausal_Logic.literal list) list *
           (Arith.nat *
             (Arith.nat Clausal_Logic.literal list)
-              CDCL_CW.conflicting_clause))));
+              CDCL_W.conflicting_clause))));
   val gene : Arith.nat -> (Arith.nat Clausal_Logic.literal list) list
   val do_all_cdcl_s : cdcl_state_inv_I -> cdcl_state_inv_I
 end = struct
@@ -1702,7 +1702,7 @@ datatype cdcl_state_inv =
         ((Arith.nat Clausal_Logic.literal list) list *
           (Arith.nat *
             (Arith.nat Clausal_Logic.literal list)
-              CDCL_CW.conflicting_clause))));
+              CDCL_W.conflicting_clause))));
 
 datatype cdcl_state_inv_I =
   ConI of
@@ -1712,7 +1712,7 @@ datatype cdcl_state_inv_I =
         ((Arith.nat Clausal_Logic.literal list) list *
           (Arith.nat *
             (Arith.nat Clausal_Logic.literal list)
-              CDCL_CW.conflicting_clause))));
+              CDCL_W.conflicting_clause))));
 
 fun gene n =
   (if Arith.equal_nata n Arith.zero_nat
@@ -1765,14 +1765,14 @@ fun find_first_unit_clause A_ (a :: l) m =
 
 fun do_propagate_step A_ s =
   (case s
-    of (m, (n, (u, (k, CDCL_CW.C_True)))) =>
+    of (m, (n, (u, (k, CDCL_W.C_True)))) =>
       (case find_first_unit_clause A_ (n @ u) m
-        of NONE => (m, (n, (u, (k, CDCL_CW.C_True))))
+        of NONE => (m, (n, (u, (k, CDCL_W.C_True))))
         | SOME (l, c) =>
           (Partial_Annotated_Clausal_Logic.Propagated (l, c) :: m,
-            (n, (u, (k, CDCL_CW.C_True)))))
-    | (m, (n, (u, (k, CDCL_CW.C_Clause ah)))) =>
-      (m, (n, (u, (k, CDCL_CW.C_Clause ah)))));
+            (n, (u, (k, CDCL_W.C_True)))))
+    | (m, (n, (u, (k, CDCL_W.C_Clause ah)))) =>
+      (m, (n, (u, (k, CDCL_W.C_Clause ah)))));
 
 fun find_conflict A_ m [] = NONE
   | find_conflict A_ m (n :: ns) =
@@ -1786,12 +1786,12 @@ fun find_conflict A_ m [] = NONE
 
 fun do_conflict_step A_ s =
   (case s
-    of (m, (n, (u, (k, CDCL_CW.C_True)))) =>
+    of (m, (n, (u, (k, CDCL_W.C_True)))) =>
       (case find_conflict A_ m (n @ u)
-        of NONE => (m, (n, (u, (k, CDCL_CW.C_True))))
-        | SOME a => (m, (n, (u, (k, CDCL_CW.C_Clause a)))))
-    | (m, (n, (u, (k, CDCL_CW.C_Clause ah)))) =>
-      (m, (n, (u, (k, CDCL_CW.C_Clause ah)))));
+        of NONE => (m, (n, (u, (k, CDCL_W.C_True))))
+        | SOME a => (m, (n, (u, (k, CDCL_W.C_Clause a)))))
+    | (m, (n, (u, (k, CDCL_W.C_Clause ah)))) =>
+      (m, (n, (u, (k, CDCL_W.C_Clause ah)))));
 
 fun do_cp_step A_ s = (do_propagate_step A_ o do_conflict_step A_) s;
 
@@ -1805,18 +1805,18 @@ fun do_cp_stepa s = Con (do_cp_step Arith.equal_nat (rough_state_of s));
 
 fun do_skip_step
   (Partial_Annotated_Clausal_Logic.Propagated (l, c) :: ls,
-    (n, (u, (k, CDCL_CW.C_Clause d))))
+    (n, (u, (k, CDCL_W.C_Clause d))))
   = (if not (List.member (Clausal_Logic.equal_literal Arith.equal_nat) d
               (Clausal_Logic.uminus_literal l)) andalso
           not (List.null d)
-      then (ls, (n, (u, (k, CDCL_CW.C_Clause d))))
+      then (ls, (n, (u, (k, CDCL_W.C_Clause d))))
       else (Partial_Annotated_Clausal_Logic.Propagated (l, c) :: ls,
-             (n, (u, (k, CDCL_CW.C_Clause d)))))
+             (n, (u, (k, CDCL_W.C_Clause d)))))
   | do_skip_step ([], va) = ([], va)
   | do_skip_step (Partial_Annotated_Clausal_Logic.Marked (vd, ve) :: vc, va) =
     (Partial_Annotated_Clausal_Logic.Marked (vd, ve) :: vc, va)
-  | do_skip_step (v, (vb, (vd, (vf, CDCL_CW.C_True)))) =
-    (v, (vb, (vd, (vf, CDCL_CW.C_True))));
+  | do_skip_step (v, (vb, (vd, (vf, CDCL_W.C_True)))) =
+    (v, (vb, (vd, (vf, CDCL_W.C_True))));
 
 fun equal_cdcl_state_inv_I sa s =
   Product_Type.equal_proda
@@ -1831,7 +1831,7 @@ fun equal_cdcl_state_inv_I sa s =
         (List.equal_list
           (List.equal_list (Clausal_Logic.equal_literal Arith.equal_nat)))
         (Product_Type.equal_prod Arith.equal_nat
-          (CDCL_CW.equal_conflicting_clause
+          (CDCL_W.equal_conflicting_clause
             (List.equal_list (Clausal_Logic.equal_literal Arith.equal_nat))))))
     (rough_state_of_I sa) (rough_state_of_I s);
 
@@ -1848,7 +1848,7 @@ fun equal_cdcl_state_inv sa s =
         (List.equal_list
           (List.equal_list (Clausal_Logic.equal_literal Arith.equal_nat)))
         (Product_Type.equal_prod Arith.equal_nat
-          (CDCL_CW.equal_conflicting_clause
+          (CDCL_W.equal_conflicting_clause
             (List.equal_list (Clausal_Logic.equal_literal Arith.equal_nat))))))
     (rough_state_of sa) (rough_state_of s);
 
@@ -1860,36 +1860,36 @@ fun do_full_cp_step s =
   end;
 
 fun maximum_level_code A_ d m =
-  CDCL_CW.get_maximum_level A_ (Multiset.Mset d) m;
+  CDCL_W.get_maximum_level A_ (Multiset.Mset d) m;
 
 fun find_level_decomp A_ m [] d k = NONE
   | find_level_decomp A_ m (l :: ls) d k =
     let
       val (i, j) =
-        (CDCL_CW.get_rev_level A_ l Arith.zero_nat (List.rev m),
+        (CDCL_W.get_rev_level A_ l Arith.zero_nat (List.rev m),
           maximum_level_code A_ (d @ ls) m);
     in
       (if Arith.equal_nata i k andalso Arith.less_nat j i then SOME (l, j)
         else find_level_decomp A_ m ls (l :: d) k)
     end;
 
-fun do_backtrack_step A_ (m, (n, (u, (k, CDCL_CW.C_Clause d)))) =
+fun do_backtrack_step A_ (m, (n, (u, (k, CDCL_W.C_Clause d)))) =
   (case find_level_decomp A_ m d [] k
-    of NONE => (m, (n, (u, (k, CDCL_CW.C_Clause d))))
+    of NONE => (m, (n, (u, (k, CDCL_W.C_Clause d))))
     | SOME (l, j) =>
-      (case bt_cut j m of NONE => (m, (n, (u, (k, CDCL_CW.C_Clause d))))
-        | SOME [] => (m, (n, (u, (k, CDCL_CW.C_Clause d))))
+      (case bt_cut j m of NONE => (m, (n, (u, (k, CDCL_W.C_Clause d))))
+        | SOME [] => (m, (n, (u, (k, CDCL_W.C_Clause d))))
         | SOME (Partial_Annotated_Clausal_Logic.Marked (_, _) :: ls) =>
           (Partial_Annotated_Clausal_Logic.Propagated (l, d) :: ls,
-            (n, (d :: u, (j, CDCL_CW.C_True))))
+            (n, (d :: u, (j, CDCL_W.C_True))))
         | SOME (Partial_Annotated_Clausal_Logic.Propagated (_, _) :: _) =>
-          (m, (n, (u, (k, CDCL_CW.C_Clause d))))))
-  | do_backtrack_step A_ (v, (vb, (vd, (vf, CDCL_CW.C_True)))) =
-    (v, (vb, (vd, (vf, CDCL_CW.C_True))));
+          (m, (n, (u, (k, CDCL_W.C_Clause d))))))
+  | do_backtrack_step A_ (v, (vb, (vd, (vf, CDCL_W.C_True)))) =
+    (v, (vb, (vd, (vf, CDCL_W.C_True))));
 
 fun do_resolve_step
   (Partial_Annotated_Clausal_Logic.Propagated (l, c) :: ls,
-    (n, (u, (k, CDCL_CW.C_Clause d))))
+    (n, (u, (k, CDCL_W.C_Clause d))))
   = (if List.member (Clausal_Logic.equal_literal Arith.equal_nat) d
           (Clausal_Logic.uminus_literal l) andalso
           (Arith.equal_nata
@@ -1899,7 +1899,7 @@ fun do_resolve_step
                (Partial_Annotated_Clausal_Logic.Propagated (l, c) :: ls))
              k orelse
             Arith.equal_nata k Arith.zero_nat)
-      then (ls, (n, (u, (k, CDCL_CW.C_Clause
+      then (ls, (n, (u, (k, CDCL_W.C_Clause
                               (List.remdups
                                 (Clausal_Logic.equal_literal Arith.equal_nat)
                                 (List.remove1
@@ -1910,12 +1910,12 @@ fun do_resolve_step
                                       Arith.equal_nat)
                                     (Clausal_Logic.uminus_literal l) d))))))
       else (Partial_Annotated_Clausal_Logic.Propagated (l, c) :: ls,
-             (n, (u, (k, CDCL_CW.C_Clause d)))))
+             (n, (u, (k, CDCL_W.C_Clause d)))))
   | do_resolve_step ([], va) = ([], va)
   | do_resolve_step (Partial_Annotated_Clausal_Logic.Marked (vd, ve) :: vc, va)
     = (Partial_Annotated_Clausal_Logic.Marked (vd, ve) :: vc, va)
-  | do_resolve_step (v, (vb, (vd, (vf, CDCL_CW.C_True)))) =
-    (v, (vb, (vd, (vf, CDCL_CW.C_True))));
+  | do_resolve_step (v, (vb, (vd, (vf, CDCL_W.C_True)))) =
+    (v, (vb, (vd, (vf, CDCL_W.C_True))));
 
 fun find_first_unused_var A_ (a :: l) m =
   (case List.find
@@ -1927,14 +1927,14 @@ fun find_first_unused_var A_ (a :: l) m =
     of NONE => find_first_unused_var A_ l m | SOME aa => SOME aa)
   | find_first_unused_var A_ [] uu = NONE;
 
-fun do_decide_step A_ (m, (n, (u, (k, CDCL_CW.C_True)))) =
+fun do_decide_step A_ (m, (n, (u, (k, CDCL_W.C_True)))) =
   (case find_first_unused_var A_ n (Partial_Annotated_Clausal_Logic.lits_of m)
-    of NONE => (m, (n, (u, (k, CDCL_CW.C_True))))
+    of NONE => (m, (n, (u, (k, CDCL_W.C_True))))
     | SOME l =>
       (Partial_Annotated_Clausal_Logic.Marked (l, Arith.suc k) :: m,
-        (n, (u, (Arith.plus_nat k Arith.one_nat, CDCL_CW.C_True)))))
-  | do_decide_step A_ (v, (vb, (vd, (vf, CDCL_CW.C_Clause vh)))) =
-    (v, (vb, (vd, (vf, CDCL_CW.C_Clause vh))));
+        (n, (u, (Arith.plus_nat k Arith.one_nat, CDCL_W.C_True)))))
+  | do_decide_step A_ (v, (vb, (vd, (vf, CDCL_W.C_Clause vh)))) =
+    (v, (vb, (vd, (vf, CDCL_W.C_Clause vh))));
 
 fun do_other_step s =
   let
@@ -1955,7 +1955,7 @@ fun do_other_step s =
                     (List.equal_list
                       (Clausal_Logic.equal_literal Arith.equal_nat)))
                   (Product_Type.equal_prod Arith.equal_nat
-                    (CDCL_CW.equal_conflicting_clause
+                    (CDCL_W.equal_conflicting_clause
                       (List.equal_list
                         (Clausal_Logic.equal_literal Arith.equal_nat))))))
               t s)
@@ -1978,7 +1978,7 @@ fun do_other_step s =
                              (List.equal_list
                                (Clausal_Logic.equal_literal Arith.equal_nat)))
                            (Product_Type.equal_prod Arith.equal_nat
-                             (CDCL_CW.equal_conflicting_clause
+                             (CDCL_W.equal_conflicting_clause
                                (List.equal_list
                                  (Clausal_Logic.equal_literal
                                    Arith.equal_nat))))))
@@ -2004,7 +2004,7 @@ Arith.equal_nat)))
                                       (List.equal_list
 (Clausal_Logic.equal_literal Arith.equal_nat)))
                                     (Product_Type.equal_prod Arith.equal_nat
-                                      (CDCL_CW.equal_conflicting_clause
+                                      (CDCL_W.equal_conflicting_clause
 (List.equal_list (Clausal_Logic.equal_literal Arith.equal_nat))))))
                                 v u)
                         then v else do_decide_step Arith.equal_nat v)
@@ -2035,17 +2035,17 @@ fun do_all_cdcl_s s =
     (if equal_cdcl_state_inv_I t s then s else do_all_cdcl_s t)
   end;
 
-end; (*struct CDCL_CW_Implementation*)
+end; (*struct CDCL_W_Implementation*)
 
 \<close>
 declare[[ML_print_depth=100]]
 ML \<open>
 open Clausal_Logic;
-open CDCL_CW_Implementation;
+open CDCL_W_Implementation;
 open Arith;
 let
   val N = gene (Nat 2)
-  val f = do_all_cdcl_s (ConI ([], (N, ([], (Nat 0, CDCL_CW.C_True)))))
+  val f = do_all_cdcl_s (ConI ([], (N, ([], (Nat 0, CDCL_W.C_True)))))
   in
 
   f
